lib/Benchmarks/TimestampSingleZeroProof.v
@@ -7,19 +7,15 @@ Notation conf := (P4automaton.configuration (P4A.interp A)).
 Notation start_left := TimestampRefZeroSingle.Start.
 Notation start_right := TimestampSpecSingle.Start.
 
-Definition r_states :=
-  Eval vm_compute in (Reachability.reachable_states
-                        A
-                        2
-                        start_left
-                        start_right).
+Definition r_states : {r : Reachability.state_pairs A & Reachability.reachable_states_wit start_left start_right r}.
+  econstructor.
+  unfold Reachability.reachable_states_wit.
+  solve_fp_wit.
+Defined.
 
 (* Definition r_len := Eval vm_compute in (length r_states).
 
 Print r_len. *)
-
-Definition top : Relations.rel conf := fun _ _ => True.
-Definition top' : Relations.rel (state_template A) := fun _ _ => True.
 
 Declare ML Module "mirrorsolve".
 
@@ -63,10 +59,10 @@ RegisterEnvCtors
                       cr_rel := btrue;
                    |} q1 q2 ->
   pre_bisimulation A
-                   (wp r_states)
-                   top
+                   (projT1 r_states)
+                   (wp (a := A))
                    []
-                   (mk_init _ _ _ _ A 2 start_left start_right)
+                   (mk_init _ _ _ _ A start_left start_right)
                    q1 q2.
 Proof.
   idtac "running timestamp single bisimulation".
