lib/Benchmarks/EdgeTransProof.v
@@ -29,12 +29,6 @@ Qed.
 
 SetSMTSolver "cvc4".
 
-Definition top : Relations.rel conf :=
-  fun q1 q2 => List.In (conf_to_state_template q1, conf_to_state_template q2) (projT1 r_states).
-
-Definition top' : Relations.rel (state_template A) :=
-  fun q1 q2 => List.In (q1, q2) (projT1 r_states).
-
 Lemma prebisim_babyip:
   forall q1 q2,
     interp_conf_rel' {| cr_st := {|
@@ -51,8 +45,8 @@ Lemma prebisim_babyip:
                       cr_rel := btrue;
                   |} q1 q2 ->
   pre_bisimulation A
-                  (wp (projT1 r_states))
-                  top
+                  (projT1 r_states)
+                  (wp (a := A))
                   []
                   (mk_init _ _ _ _ A start_left start_right)
                   q1 q2.
@@ -66,14 +60,12 @@ Proof.
   unfold mk_init.
   rewrite Hr.
   clear Hr.
-  
+
   set (rel0 := (List.nodup _) (mk_partition _ _ _ _ _ _)).
   vm_compute in rel0.
   subst rel0.
-  
-  time "build phase" repeat (time "single step" run_bisim top top' (projT1 r_states)).
 
+  time "build phase" repeat (time "single step" run_bisim).
   print_rel_len.
-  (* run_bisim top top' r_states. *)
-  time "close phase" close_bisim top'.
+  time "close phase" close_bisim.
 Time Admitted.
